remove  hypothesis on set in wf_universe

template-coq/theories/Typing.v
@@ -814,7 +814,18 @@ Definition wf_cofixpoint (Σ : global_env) mfix :=
 
 Definition wf_universe Σ s := 
     forall l, UnivExprSet.In l (Universe.lvl s) -> 
-      Level.is_set (UnivExpr.get_level l) \/ LevelSet.In (UnivExpr.get_level l) (global_ext_levels Σ).
+      LevelSet.In (UnivExpr.get_level l) (global_ext_levels Σ).
+
+Lemma global_ext_levels_Set Σ : LevelSet.In Level.lSet (global_ext_levels Σ).
+Proof.
+  apply LevelSetProp.Dec.F.union_3, LevelSetProp.Dec.F.mem_2, global_levels_Set.
+Qed.
+
+(* FixMe: Adapt to local sorts *)
+Lemma wf_universe_Set Σ s : Universe.lvl s = UnivLevel.set -> wf_universe Σ s.
+Proof.
+  move: s=> [??] /= -> ? /UnivExprSetFact.singleton_iff <- /=; apply global_ext_levels_Set.
+Qed.
 
 Reserved Notation "'wf_local' Σ Γ " (at level 9, Σ, Γ at next level).
 
@@ -1045,17 +1056,14 @@ Hint Resolve typing_wf_local : wf.
 Lemma type_Prop `{checker_flags} Σ :
   Σ ;;; [] |- tSort Universe.lProp : tSort Universe.type1.
 Proof.
-  change (  Σ ;;; [] |- tSort (Universe.lProp) : tSort Universe.type1);
-  constructor;first constructor.
-  move=> ? /=; rewrite UnivExprSetFact.singleton_iff=> <-; by left.
+  constructor;first constructor; by apply wf_universe_Set.
 Defined.
 
 Lemma type_Prop_wf `{checker_flags} Σ Γ :
   wf_local Σ Γ ->
   Σ ;;; Γ |- tSort Universe.lProp : tSort Universe.type1.
 Proof. 
-  constructor ;auto.
-  move=> ? /=; rewrite UnivExprSetFact.singleton_iff=> <-; by left.
+  constructor ;auto. by apply wf_universe_Set.
 Defined.
 
 Definition env_prop `{checker_flags} (P : forall Σ Γ t T, Type) (PΓ : forall Σ Γ (wfΓ : wf_local Σ Γ), Type):=
